wip

RemoveScopedVarsProof.dfy
@@ -1,5 +1,5 @@
 include "BoogieSemantics.dfy"
-include "MakeScopedVarsUniqueImpl.dfy"
+include "DesugarScopedVarsImpl.dfy"
 include "Naming.dfy"
 include "dafny-libraries/src/Collections/Sequences/Seq.dfy"
 include "dafny-libraries/src/Collections/Maps/Maps.dfy"
@@ -12,18 +12,140 @@ module MakeScopedVarsUniqueProof {
   import Maps
   import Util
   import opened Wrappers
-  import opened MakeScopedVarsUniqueImpl
+  import opened DesugarScopedVarsImpl
   import opened Naming
 
-  lemma RelStateRemoveScopedVarsCorrect<A(!new)>(a: absval_interp<A>, c: Cmd, post: WpPost<A>)
-    requires 
-      var (c', decls) := RemoveScopedVars(c);
-      LabelsWellDefAux(c, post.scopes.Keys) && LabelsWellDefAux(c', post.scopes.Keys)
+  //predicate StatesAgreeOnSet<A(!new)>(s1: state<A>, s2: state<A>, 
+  predicate PredDepend<A(!new)>(p: Predicate<A>, depVars: set<var_name>)
+  {
+    forall s1, s2 | 
+      (forall x | x in depVars :: Maps.Get(s1, x) == Maps.Get(s2, x)) :: 
+      p(s1) == p(s2)
+  }
+
+  predicate PostDepend<A(!new)>(post: WpPost<A>, depVars: set<var_name>)
+  {
+    && PredDepend(post.normal, depVars)
+    && PredDepend(post.currentScope, depVars)
+    && (forall lbl | lbl in post.scopes.Keys :: PredDepend(post.scopes[lbl], depVars))
+  }
+
+  lemma {:verify false} RemoveScopedVarsPreserveWf(c: Cmd, activeVars: set<var_name>)
+    requires c.WellFormedVars(activeVars)
     ensures 
       var (c', decls) := RemoveScopedVars(c);
-      forall s :: WpCmd(a, c, post)(s) == ForallVarDecls(a, decls, WpCmd(a, c', ResetVarsPost(decls, post, s)))(s)
-    /* almost the same as Scope(None, decls, body)
-      Main difference is that currentScope is not updated.
-      If show that body has no direct breaks, then it would be the same
-    */
+      c'.WellFormedVars(activeVars+GetVarNames(decls))
+  {
+    var (c', decls) := RemoveScopedVars(c);
+    match c
+    case SimpleCmd(sc) => SimpleCmdWellFormedVarsLarger(sc, activeVars, activeVars+GetVarNames(decls));
+    case Break(_) => 
+    case Scope(optLabel, varDecls, body) => 
+      var (body', declsBody) := RemoveScopedVars(body);
+      assert body'.WellFormedVars((activeVars+GetVarNames(varDecls))+GetVarNames(declsBody)) by {
+        RemoveScopedVarsPreserveWf(body, activeVars+GetVarNames(varDecls));
+      }
+
+      calc {
+        (activeVars+GetVarNames(varDecls))+GetVarNames(declsBody);
+        activeVars+(GetVarNames(varDecls)+GetVarNames(declsBody));
+        activeVars+GetVarNames(varDecls+declsBody);
+      }
+
+      assert body'.WellFormedVars(activeVars+GetVarNames(varDecls+declsBody));
+
+      calc {
+        c'.WellFormedVars(activeVars+GetVarNames(decls));
+        body'.WellFormedVars((activeVars+GetVarNames(varDecls+declsBody))+GetVarNames([]));
+        { assert GetVarNames([]) == {}; }
+        body'.WellFormedVars((activeVars+GetVarNames(varDecls+declsBody))+{});
+        { assert (activeVars+GetVarNames(varDecls+declsBody))+{} == activeVars+GetVarNames(varDecls+declsBody); }
+        body'.WellFormedVars(activeVars+GetVarNames(varDecls+declsBody));
+      }
+    case If(None, thn, els) => 
+      var (thn', declsThn) := RemoveScopedVars(thn);
+      var (els', declsEls) := RemoveScopedVars(els);
+
+      assert 
+        && thn'.WellFormedVars(activeVars+GetVarNames(declsThn))
+        && els'.WellFormedVars(activeVars+GetVarNames(declsEls));
+
+      assert GetVarNames(decls) == GetVarNames(declsThn)+GetVarNames(declsEls);
+
+      CmdWellFormedVarsLarger(thn', activeVars+GetVarNames(declsThn), activeVars+GetVarNames(decls));
+      CmdWellFormedVarsLarger(els', activeVars+GetVarNames(declsEls), activeVars+GetVarNames(decls));
+    case Seq(c1, c2) =>
+      var (c1', decls1) := RemoveScopedVars(c1);
+      var (c2', decls2) := RemoveScopedVars(c2);
+
+      CmdWellFormedVarsLarger(c1', activeVars+GetVarNames(decls1), activeVars+GetVarNames(decls));
+      CmdWellFormedVarsLarger(c2', activeVars+GetVarNames(decls2), activeVars+GetVarNames(decls));
+    case _ => assume false;
+  }
+
+  lemma RemoveScopedVarsCorrect<A(!new)>(a: absval_interp<A>, activeVars: set<var_name>, c: Cmd, post: WpPost<A>)
+    requires 
+      var (c', decls) := RemoveScopedVars(c);
+      && LabelsWellDefAux(c, post.scopes.Keys) 
+      && LabelsWellDefAux(c', post.scopes.Keys) 
+      && c.WellFormedVars(activeVars) 
+      && PostDepend(post, activeVars)
+      && activeVars !! GetVarNames(decls)
+    ensures 
+      var (c', decls) := RemoveScopedVars(c);
+      forall s :: WpCmd(a, c, post)(s) == ForallVarDecls(a, decls, WpCmd(a, c', post))(s)
+    {
+      var (c', decls) := RemoveScopedVars(c);
+      assert c'.WellFormedVars(activeVars+GetVarNames(decls)) by {
+        RemoveScopedVarsPreserveWf(c, activeVars);
+      }
+
+      forall s | true
+      ensures WpCmd(a, c, post)(s) == ForallVarDecls(a, decls, WpCmd(a, c', post))(s)
+      {
+        match c 
+        case SimpleCmd(sc) => ForallVarDeclsEmpty(a, WpCmd(a, c', post)); 
+        case Break(_) => ForallVarDeclsEmpty(a, WpCmd(a, c', post)); 
+        case Scope(_, varDecls, body) => assume false;
+        case If(None, thn, els) => assume false;
+        case Seq(c1, c2) => 
+          // WpPost(WpCmd(a, c2, post), post.currentScope, post.scopes)
+          var (c1', decls1) := RemoveScopedVars(c1);
+          var (c2', decls2) := RemoveScopedVars(c2);
+
+          var post2 := WpPost(WpCmd(a, c2, post), post.currentScope, post.scopes);
+          var post2' := WpPost(ForallVarDecls(a, decls2, WpCmd(a, c2',post)), post.currentScope, post.scopes);
+          var post2NoQuant' := WpPost(WpCmd(a, c2',post), post.currentScope, post.scopes);
+
+          calc {
+            WpCmd(a, Seq(c1, c2), post)(s);
+            { reveal WpCmd(); }
+            WpCmd(a, c1, post2)(s);
+            { 
+              assert c2'.WellFormedVars(activeVars+GetVarNames(decls2)) by {
+                RemoveScopedVarsPreserveWf(c2, activeVars);
+              }
+              RemoveScopedVarsCorrect(a, activeVars, c2, post); 
+              WpCmdPointwise(a, c1, post2, post2', s);
+            }
+            WpCmd(a, c1, post2')(s);
+            { assume false; RemoveScopedVarsCorrect(a, activeVars, c1, post2'); }
+            ForallVarDecls(a, decls1, WpCmd(a, c1', post2'))(s);
+            { assume false; }
+            ForallVarDecls(a, decls1, ForallVarDecls(a, decls2, WpCmd(a, c1', post2NoQuant')))(s);
+            { assume false; }
+            ForallVarDecls(a, decls1+decls2, WpCmd(a, c1', post2NoQuant'))(s);
+            { assume false; }
+            ForallVarDecls(a, decls1+decls2, WpCmd(a, Seq(c1', c2'), post))(s);
+          }
+        case _ => assume false;
+      }
+
+      /* these reveal statements are needed due to a bug 
+        (see https://github.com/dafny-lang/dafny/issues/2260) 
+      */
+      reveal WpCmd();
+      reveal ForallVarDecls();
+      
+    } 
 }
